Add condition to wpr that must hold at start of each execution.

src/program_logic/recovery_weakestpre.v
@@ -17,23 +17,28 @@ Class perennialG (Λ : language) (CS: crash_semantics Λ) (T: ofeT) (Σ : gFunct
 
 Definition wpr_pre `{perennialG Λ CS T Σ} (s : stuckness) (k: nat)
     (wpr : invG Σ -d> crashG Σ -d> pbundleG T Σ -d> coPset -d> expr Λ -d> expr Λ -d> (val Λ -d> iPropO Σ) -d>
+                     (invG Σ -d> pbundleG T Σ -d> iPropO Σ) -d>
                      (invG Σ -d> pbundleG T Σ -d> val Λ -d> iPropO Σ) -d> iPropO Σ) :
-  invG Σ -d> crashG Σ -d> pbundleG T Σ -d> coPset -d> expr Λ -d> expr Λ -d> (val Λ -d> iPropO Σ) -d> (invG Σ -d> pbundleG T Σ -d> val Λ -d> iPropO Σ) -d> iPropO Σ :=
-  λ H1 H2 t E e rec Φ Φr,
+  invG Σ -d> crashG Σ -d> pbundleG T Σ -d> coPset -d> expr Λ -d> expr Λ -d> (val Λ -d> iPropO Σ) -d>
+  (invG Σ -d> pbundleG T Σ -d> iPropO Σ) -d>
+  (invG Σ -d> pbundleG T Σ -d> val Λ -d> iPropO Σ) -d> iPropO Σ :=
+  λ H1 H2 t E e rec Φ Φinv Φr,
   (WPC e @ s ; k; E ; ∅
      {{ Φ }}
      {{ ∀ σ σ' (HC: crash_prim_step CS σ σ') κs n,
-        state_interp σ κs n ={∅}=∗  ▷ ∀ H1 H2, NC -∗ ∃ t, state_interp σ' κs 0 ∗ wpr H1 H2 t E rec rec (λ v, Φr H1 t v) Φr ∗ NC}})%I.
+        state_interp σ κs n ={∅}=∗  ▷ ∀ H1 H2, NC -∗ ∃ t, state_interp σ' κs 0 ∗ (Φinv H1 t ∧ wpr H1 H2 t E rec rec (λ v, Φr H1 t v) Φinv Φr) ∗ NC}})%I.
 
 Local Instance wpr_pre_contractive `{!perennialG Λ CS T Σ} s k: Contractive (wpr_pre s k).
 Proof.
-  rewrite /wpr_pre=> n wp wp' Hwp ?? t E1 e1 rec Φ Φc.
+  rewrite /wpr_pre=> n wp wp' Hwp ?? t E1 e1 rec Φ Φinv Φc.
   apply wpc_ne; eauto;
   repeat (f_contractive || f_equiv). apply Hwp.
 Qed.
 
 Definition wpr_def `{!perennialG Λ CS T Σ} (s : stuckness) k :
-  invG Σ → crashG Σ → pbundleG T Σ → coPset → expr Λ → expr Λ → (val Λ → iProp Σ) → (invG Σ → pbundleG T Σ → val Λ → iProp Σ) → iProp Σ := fixpoint (wpr_pre s k).
+  invG Σ → crashG Σ → pbundleG T Σ → coPset → expr Λ → expr Λ → (val Λ → iProp Σ) →
+  (invG Σ → pbundleG T Σ → iProp Σ) →
+  (invG Σ → pbundleG T Σ → val Λ → iProp Σ) → iProp Σ := fixpoint (wpr_pre s k).
 Definition wpr_aux `{!perennialG Λ CS T Σ} : seal (@wpr_def Λ CS T Σ _). by eexists. Qed.
 Definition wpr `{!perennialG Λ CS T Σ} := wpr_aux.(unseal).
 Definition wpr_eq `{!perennialG Λ CS T Σ} : wpr = @wpr_def Λ CS T Σ _ := wpr_aux.(seal_eq).
@@ -48,17 +53,17 @@ Implicit Types Φc : invG Σ → pbundleG T Σ → val Λ → iProp Σ.
 Implicit Types v : val Λ.
 Implicit Types e : expr Λ.
 
-Lemma wpr_unfold s k Hi Hc t E e rec Φ Φc :
-  wpr s k Hi Hc t E e rec Φ Φc ⊣⊢ wpr_pre s k (wpr s k) Hi Hc t E e rec Φ Φc.
+Lemma wpr_unfold s k Hi Hc t E e rec Φ Φinv Φc :
+  wpr s k Hi Hc t E e rec Φ Φinv Φc ⊣⊢ wpr_pre s k (wpr s k) Hi Hc t E e rec Φ Φinv Φc.
 Proof. rewrite wpr_eq. apply (fixpoint_unfold (wpr_pre s k)). Qed.
 
 (* There's a stronger version of this *)
-Lemma wpr_strong_mono s k Hi Hc t E e rec Φ Ψ Φr Ψr :
-  wpr s k Hi Hc t E e rec Φ Φr -∗
-  (∀ v, Φ v ==∗ Ψ v) ∧ (∀ Hi t v, Φr Hi t v ==∗ Ψr Hi t v) -∗
-  wpr s k Hi Hc t E e rec Ψ Ψr.
+Lemma wpr_strong_mono s k Hi Hc t E e rec Φ Ψ Φinv Ψinv Φr Ψr :
+  wpr s k Hi Hc t E e rec Φ Φinv Φr -∗
+  (∀ v, Φ v ==∗ Ψ v) ∧ (∀ Hi t, Φinv Hi t -∗ Ψinv Hi t) ∧ (∀ Hi t v, Φr Hi t v ==∗ Ψr Hi t v) -∗
+  wpr s k Hi Hc t E e rec Ψ Ψinv Ψr.
 Proof.
-  iIntros "H HΦ". iLöb as "IH" forall (e t Hi Hc E Φ Ψ Φr Ψr).
+  iIntros "H HΦ". iLöb as "IH" forall (e t Hi Hc E Φ Ψ Φinv Ψinv Φr Ψr).
   rewrite ?wpr_unfold /wpr_pre.
   iApply (wpc_strong_mono' with "H") ; auto.
   iSplit.
@@ -67,18 +72,25 @@ Proof.
   rewrite difference_diag_L.
   iModIntro. iIntros (?????) "Hinterp". iMod ("H" with "[//] Hinterp") as "H".
   iModIntro. iNext. iIntros (Hi' Hc') "HNC". iDestruct ("H" $! Hi' Hc' with "[$]") as (?) "(?&H&HNC)".
-  iExists _. iFrame. iApply ("IH" with "[$]").
-  iSplit; iIntros; iDestruct ("HΦ") as "(_&H)"; by iMod ("H" with "[$]").
+  iExists _. iFrame.
+  iSplit.
+  - iDestruct "H" as "(H&_)". iDestruct "HΦ" as "(_&HΦ&_)". by iApply "HΦ".
+  - iDestruct "H" as "(_&H)".
+    iApply ("IH" with "[$]").
+    iSplit; [| iSplit].
+    * iIntros. iDestruct ("HΦ") as "(_&_&H)"; by iMod ("H" with "[$]").
+    * iDestruct ("HΦ") as "(_&$&_)"; auto.
+    * iIntros. iDestruct ("HΦ") as "(_&_&H)"; by iMod ("H" with "[$]").
 Qed.
 
 (* To prove a recovery wp for e with rec, it suffices to prove a crash wp for e,
    where the crash condition implies the precondition for a crash wp for rec *)
-Lemma idempotence_wpr s k E e rec Φx Φrx Φcx Hi Hc t:
+Lemma idempotence_wpr s k E e rec Φx Φinv Φrx Φcx Hi Hc t:
   ((WPC e @ s ; k ; E ; ∅ {{ Φx t }} {{ Φcx t }}) -∗
    (□ ∀ (H: invG Σ) (Hc: crashG Σ) (t: pbundleG T Σ) σ σ' (HC: crash_prim_step CS σ σ') κs n,
         Φcx t -∗ state_interp σ κs n ={∅}=∗
-        ▷ ∀ H' (Hc': crashG Σ), NC -∗ ∃ t', state_interp σ' κs 0 ∗ WPC rec @ s ; k; E ; ∅ {{ Φrx H' t' }} {{ Φcx t' }} ∗ NC) -∗
-    wpr s k Hi Hc t E e rec (Φx t) Φrx)%I.
+        ▷ ∀ H' (Hc': crashG Σ), NC -∗ ∃ t', state_interp σ' κs 0 ∗ (Φinv H' t' ∧ WPC rec @ s ; k; E ; ∅ {{ Φrx H' t' }} {{ Φcx t' }}) ∗ NC) -∗
+    wpr s k Hi Hc t E e rec (Φx t) Φinv Φrx)%I.
 Proof.
   iLöb as "IH" forall (E e Hi Hc t Φx).
   iIntros "He #Hidemp".
@@ -91,6 +103,9 @@ Proof.
   { eauto. }
   iModIntro. iNext. iIntros (Hi' Hc') "HNC". iDestruct ("H" $! Hi' Hc' with "[$]") as (t') "(?&Hc&HNC)".
   iExists _. iFrame.
+  iSplit.
+  { iDestruct "Hc" as "($&_)". }
+  iDestruct "Hc" as "(_&Hc)".
   iApply ("IH" $! E rec Hi' Hc' t' (λ t v, Φrx Hi' t v)%I with "[Hc]").
   { iApply (wpc_strong_mono' with "Hc"); rewrite ?difference_diag_L; auto. }
   eauto.
